factored out type desriptions from the fixtree type

theories/Ref/FixTree.v
@@ -39,400 +39,15 @@ Import Monads.
 Import ProperNotations.
 
 
-(***
- *** List utilities
- ***)
-
-(* A version of nth_default that does primary recursion on the list *)
-Fixpoint nth_default' {A} (d : A) (l : list A) n : A :=
-  match l with
-  | nil => d
-  | cons x l' => match n with
-                 | 0 => x
-                 | S n' => nth_default' d l' n'
-                 end
-  end.
-
-(* Reverse the first list and append the second *)
-Fixpoint rev_app {A} (l1 l2 : list A) : list A :=
-  match l1 with
-  | nil => l2
-  | cons x l1' => rev_app l1' (cons x l2)
-  end.
-
-(* Reverse and prepend each list in a list of lists *)
-Fixpoint revs_app {A} (ls : list (list A)) (l2 : list A) : list A :=
-  match ls with
-  | nil => l2
-  | cons l1 ls' => rev_app l1 (revs_app ls' l2)
-  end.
-
-(* Delete the nth element of a list *)
-Fixpoint deleteNth {A} n (l : list A) {struct l} : list A :=
-  match l with
-  | nil => nil
-  | cons a l' => match n with
-                 | 0 => l'
-                 | S n' => cons a (deleteNth n' l')
-                 end
-  end.
-
-(* Insert an element at the nth position in a list, or at the end if n is too big *)
-Fixpoint insertNth {A} (a:A) n l {struct n} : list A :=
-  match n with
-  | 0 => a :: l
-  | S n' => match l with
-            | nil => a :: nil
-            | b :: l' => b :: insertNth a n' l'
-            end
-  end.
-
-(* Drop the first n elements of a list *)
-Fixpoint drop {A} n (l:list A) {struct n} : list A :=
-  match n with
-  | 0 => l
-  | S n' => match l with
-            | nil => nil
-            | _ :: l' => drop n' l'
-            end
-  end.
-
-
-(* A proof that x is the nth element of a list *)
-Inductive isNth {A} (a:A) : nat -> list A -> Prop :=
-| isNth_base l : isNth a 0 (cons a l)
-| isNth_cons n x l : isNth a n l -> isNth a (S n) (cons x l).
-
-Lemma not_isNth_nil {A} (a:A) n : isNth a n nil -> False.
-Proof.
-  induction n; intros; inversion H.
-Qed.
-
-Lemma isNthHead {A} {a:A} {b l} (isn : isNth a 0 (cons b l)) : a = b.
-Proof.
-  inversion isn. reflexivity.
-Qed.
-
-Lemma isNthTail {A} {a:A} {n b l} (isn : isNth a (S n) (cons b l)) : isNth a n l.
-Proof.
-  inversion isn. assumption.
-Qed.
-
-Lemma isNthEq {A} {a b:A} {n l} (isn_a : isNth a n l) (isn_b : isNth b n l) : a = b.
-Proof.
-  revert isn_b; induction isn_a; intros; inversion isn_b.
-  - reflexivity.
-  - apply IHisn_a; assumption.
-Qed.
-
-Definition isNthDelete {A} {a:A} {n l} (isn: isNth a n l) m :
-  (m = n) + { n' | isNth a n' (deleteNth m l) }.
-Proof.
-  revert m l isn; induction n; intros; destruct l.
-  - elimtype False; inversion isn.
-  - destruct m; [ left; reflexivity | ]. right. exists 0. inversion isn. constructor.
-  - elimtype False; inversion isn.
-  - destruct m; [ right; exists n; eapply isNthTail; eassumption | ].
-    destruct (IHn m l (isNthTail isn)).
-    + left; subst m; reflexivity.
-    + right; destruct s. exists (S x). econstructor; eassumption.
-Defined.
-
-Definition isNthUnInsert {A} {a:A} {b n m l}
-  (isn: isNth a n (insertNth b m l)) : (a = b) + { n' | isNth a n' l }.
-Proof.
-  revert m l isn; induction n; intros.
-  - destruct m; [ left; inversion isn; reflexivity | ].
-    destruct l; [ left; inversion isn; reflexivity | ].
-    right. exists 0. inversion isn. constructor.
-  - destruct m.
-    + right; exists n. inversion isn. assumption.
-    + destruct l; [ elimtype False; inversion isn; inversion H1 | ].
-      destruct (IHn m l (isNthTail isn)); [ left; assumption | ].
-      destruct s. right; exists (S x); constructor; assumption.
-Qed.
-
-
-(* Build the right-nested tuple type of a list of types formed by mapping a
-function across a list *)
-Polymorphic Fixpoint mapTuple@{u v} {T:Type@{v}} (f : T -> Type@{u}) (xs : list T) : Type@{u} :=
-  match xs with
-  | nil => unit
-  | cons x xs' => f x * mapTuple f xs'
-  end.
-
-Polymorphic Fixpoint mapMapTuple@{u v} {T:Type@{v}} {f g : T -> Type@{u}}
-  (fg : forall t, f t -> g t) (xs : list T) : mapTuple f xs -> mapTuple g xs :=
-  match xs return mapTuple f xs -> mapTuple g xs with
-  | nil => fun u => u
-  | cons x xs' => fun tup => (fg x (fst tup), mapMapTuple fg xs' (snd tup))
-  end.
-
-(* Append two mapTuple tuples *)
-Polymorphic Fixpoint appMapTuple@{u v} {T:Type@{v}} {f : T -> Type@{u}} (xs ys : list T) :
-  mapTuple f xs -> mapTuple f ys -> mapTuple f (app xs ys) :=
-  match xs return mapTuple f xs -> mapTuple f ys -> mapTuple f (app xs ys) with
-  | nil => fun _ tup2 => tup2
-  | cons x xs' =>
-      fun tup1 tup2 => (fst tup1, appMapTuple xs' ys (snd tup1) tup2)
-  end.
-
-(* Split a mapTuple on an append in two *)
-Polymorphic Fixpoint splitMapTuple@{u v} {T:Type@{v}} {f : T -> Type@{u}} {xs ys : list T} :
-  mapTuple f (app xs ys) -> mapTuple f xs * mapTuple f ys :=
-  match xs return mapTuple f (app xs ys) -> mapTuple f xs * mapTuple f ys with
-  | nil => fun tup => (tt, tup)
-  | cons x xs' =>
-      fun tup => ((fst tup, fst (splitMapTuple (snd tup))),
-                   snd (splitMapTuple (snd tup)))
-  end.
-
-(* Drop the first n elements from a mapTuple *)
-Polymorphic Fixpoint dropMapTuple@{u v} {T:Type@{v}} {f : T -> Type@{u}}
-  n {xs : list T} : mapTuple f xs -> mapTuple f (drop n xs) :=
-  match n return mapTuple f xs -> mapTuple f (drop n xs) with
-  | 0 => fun tup => tup
-  | S n' =>
-      match xs return mapTuple f xs -> mapTuple f (drop (S n') xs) with
-      | nil => fun tup => tup
-      | _ :: xs' => fun tup => dropMapTuple n' (snd tup)
-      end
-  end.
-
-(* Project the nth element of a mapTuple, using a default if n is too big *)
-Polymorphic Fixpoint nthProjDefault@{u v} {T:Type@{v}} {f : T -> Type@{u}} {dT:T} (d:f dT) {xs}
-  : forall n, mapTuple f xs -> f (nth_default' dT xs n) :=
-  match xs return forall n, mapTuple f xs -> f (nth_default' dT xs n) with
-  | nil => fun _ _ => d
-  | cons x xs' =>
-      fun n =>
-        match n return mapTuple f (cons x xs') -> f (nth_default' dT (cons x xs') n) with
-        | 0 => fun tup => fst tup
-        | S n' => fun tup => nthProjDefault d n' (snd tup)
-        end
-  end.
-
-
-Polymorphic Fixpoint nthProj@{u v} {T:Type@{v}} {f : T -> Type@{u}} {t n} :
-  forall {l}, isNth t n l -> mapTuple f l -> f t.
-Proof.
-  induction n; intro l; destruct l; intros isn mtup.
-  - elimtype False; inversion isn.
-  - destruct mtup. rewrite (isNthHead isn). assumption.
-  - elimtype False; inversion isn.
-  - destruct mtup. apply (IHn l (isNthTail isn) m).
-Defined.
-
-
-(*
-Polymorphic Fixpoint nthProj@{u v} {T:Type@{v}} (f : T -> Type@{u}) t n :
-  forall l, isNth t n l -> mapTuple f l -> f t :=
-  match n return forall l, isNth t n l -> mapTuple f l -> f t with
-  | 0 => fun l =>
-           match l return isNth t 0 l -> mapTuple f l -> f t with
-           | nil => fun isn => match not_isNth_nil t 0 isn with end
-           | cons b l' =>
-               fun isn 
-  end.
-*)
-
-
-(**
- ** List Inclusions
- **)
-
-(* A single step of list inclusion, which adds an element into a list; note that
-this in in Type, not in Prop, because we care about the contents *)
-Inductive listIncl1 {A} : list A -> list A -> Type :=
-| incl1Base a l2 : listIncl1 l2 (cons a l2)
-| incl1Step a l1 l2 : listIncl1 l1 l2 -> listIncl1 (cons a l1) (cons a l2)
-.
-
-(* Map an index through a single step of list inclusion *)
-Fixpoint applyListIncl1 {A l1 l2} (incl: @listIncl1 A l1 l2) n : nat :=
-  match incl with
-  | incl1Base _ _ => S n
-  | incl1Step _ l1' l2' incl' =>
-      match n with
-      | 0 => 0
-      | S n' => S (applyListIncl1 incl' n')
-      end
-  end.
-
-(* Map an isNth proof through a single step of list inclusion *)
-Lemma applyListIncl1Nth {A l1 l2} (incl: @listIncl1 A l1 l2) a n :
-  isNth a n l1 -> isNth a (applyListIncl1 incl n) l2.
-Proof.
-  revert n; induction incl; intros; [ | destruct n ].
-  - constructor; assumption.
-  - inversion H. constructor.
-  - constructor. apply IHincl. inversion H. assumption.
-Qed.
-
-(* This is the reflexive-transitive closure of listIncl1, except we need it in
-Type, not Prop, because we care about the contents *)
-Inductive listIncl {A} : list A -> list A -> Type :=
-| reflListIncl l : listIncl l l
-| stepListIncl {l1 l2} (incl: listIncl1 l1 l2) : listIncl l1 l2
-| compListIncl {l1 l2 l3} (incl1 : listIncl l1 l2) (incl2 : listIncl l2 l3)
-  : listIncl l1 l3
-.
-
-Fixpoint applyListIncl {A l1 l2} (incl: @listIncl A l1 l2) : nat -> nat :=
-  match incl with
-  | reflListIncl _ => fun n => n
-  | stepListIncl incl1 => applyListIncl1 incl1
-  | compListIncl incl1 incl2 => fun n => applyListIncl incl2 (applyListIncl incl1 n)
-  end.
-
-Fixpoint applyListInclNth {A l1 l2} (incl: @listIncl A l1 l2) :
-  forall {a n}, isNth a n l1 -> isNth a (applyListIncl incl n) l2 :=
-  match incl in listIncl l1 l2
-        return forall a n, isNth a n l1 ->
-                           isNth a (applyListIncl incl n) l2 with
-  | reflListIncl _ => fun _ _ isn => isn
-  | stepListIncl incl1 => applyListIncl1Nth incl1
-  | compListIncl incl1 incl2 =>
-      fun a n isn => applyListInclNth incl2 (applyListInclNth incl1 isn)
-  end.
-
-(* Build an inclusion from nil into any list *)
-Fixpoint nilListIncl {A} (l:list A) : listIncl nil l :=
-  match l return listIncl nil l with
-  | nil => reflListIncl nil
-  | a :: l' => compListIncl (nilListIncl l') (stepListIncl (incl1Base a l'))
-  end.
-
-(* Prefix a listIncl1 with a single element that stays constant *)
-Definition consListIncl1 {A} (a:A) {l1 l2} (incl : listIncl1 l1 l2) :
-  listIncl1 (cons a l1) (cons a l2) :=
-  incl1Step a _ _ incl.
-
-(* Prefix a listIncl with a single element that stays constant *)
-Fixpoint consListIncl {A} (a:A) {l1 l2} (incl : listIncl l1 l2) :
-  listIncl (cons a l1) (cons a l2) :=
-  match incl in listIncl l1 l2 return listIncl (cons a l1) (cons a l2) with
-  | reflListIncl l => reflListIncl (cons a l)
-  | stepListIncl incl1 => stepListIncl (consListIncl1 a incl1)
-  | compListIncl incl1 incl2 =>
-      compListIncl (consListIncl a incl1) (consListIncl a incl2)
-  end.
-
-(* Cons an element onto the right side of a listIncl *)
-Definition consListInclR {A} (a:A) {l1 l2} (incl : listIncl l1 l2)
-  : listIncl l1 (cons a l2) :=
-  compListIncl incl (stepListIncl (incl1Base a l2)).
-
-(* Un-cons an element onto the right side of a listIncl *)
-Definition consListInclL {A} (a:A) {l1 l2} (incl : listIncl (cons a l1) l2)
-  : listIncl l1 l2 :=
-  compListIncl (stepListIncl (incl1Base a l1)) incl.
-
-
-Definition pushoutListIncl1 {A} {l1 l2 l3}
-  (incl1 : listIncl1 l1 l2) (incl2 : listIncl1 l1 l3) :
-  { l4:list A & listIncl1 l2 l4 & listIncl1 l3 l4 }.
-Proof.
-  revert l3 incl2; induction incl1; intros; [ | inversion incl2 ].
-  - exists (a :: l3); [ apply (incl1Step a _ _ incl2) | apply incl1Base ].
-  - subst l3. subst l0. exists (a0 :: a :: l2); [ apply incl1Base | ].
-    eapply incl1Step; eapply incl1Step; eassumption.
-  - subst l3. subst a0. subst l0.
-    destruct (IHincl1 l4 X) as [ l5 incl1' incl2' ].
-    exists (a :: l5); eapply incl1Step; eassumption.
-Qed.
-
-Definition pushoutListInclOne {A} {l1 l2 l3}
-  (incl1 : listIncl1 l1 l2) (incl2 : listIncl l1 l3) :
-  { l4:list A & listIncl l2 l4 & listIncl1 l3 l4 }.
-Proof.
-  revert l2 incl1; induction incl2; intros.
-  - exists l2; [ constructor | assumption ].
-  - destruct (pushoutListIncl1 incl incl1) as [ l4 incl1' incl2' ].
-    exists l4; [ apply stepListIncl | ]; assumption.
-  - destruct (IHincl2_1 l0 incl1) as [ l4 incl1' incl2' ].
-    destruct (IHincl2_2 _ incl2') as [ l5 incl1'' incl2'' ].
-    exists l5; [ | assumption ].
-    eapply compListIncl; eassumption.
-Defined.
-
-Definition pushoutListIncl {A} {l1 l2 l3}
-  (incl1 : listIncl l1 l2) (incl2 : listIncl l1 l3) :
-  { l4:list A & listIncl l2 l4 & listIncl l3 l4 }.
-Proof.
-  revert l3 incl2; induction incl1; intros.
-  - exists l3; try assumption; constructor.
-  - destruct (pushoutListInclOne incl incl2) as [ l4 incl1' incl2' ].
-    exists l4; try assumption; apply stepListIncl; assumption.
-  - destruct (IHincl1_1 l0 incl2) as [ l4 incl1' incl2' ].
-    destruct (IHincl1_2 l4 incl1') as [ l5 incl1'' incl2'' ].
-    exists l5; [ assumption | eapply compListIncl; eassumption ].
-Defined.
-
-Definition pushoutListInclList {A l1 l2 l3}
-  (incl1 : listIncl l1 l2) (incl2 : listIncl l1 l3) : list A :=
-  match pushoutListIncl incl1 incl2 with
-  | existT2 _ _ l _ _ => l
-  end.
-
-Definition pushoutListInclIncl1 {A l1 l2 l3}
-  (incl1 : listIncl l1 l2) (incl2 : listIncl l1 l3)
-  : @listIncl A l2 (pushoutListInclList incl1 incl2) :=
-  projT2 (sigT_of_sigT2 (pushoutListIncl incl1 incl2)).
-
-Definition pushoutListInclIncl2 {A l1 l2 l3}
-  (incl1 : listIncl l1 l2) (incl2 : listIncl l1 l3)
-  : @listIncl A l3 (pushoutListInclList incl1 incl2) :=
-  projT3 (pushoutListIncl incl1 incl2).
-
-
-Definition deleteNthIncl {A} n (l:list A) : listIncl (deleteNth n l) l.
-Proof.
-  revert n; induction l; intros; [ | destruct n ].
-  - apply reflListIncl.
-  - apply stepListIncl; apply incl1Base.
-  - apply consListIncl. apply IHl.
-Defined.
-
-Definition undeleteIncl {A l1 l2 n} (incl : @listIncl A (deleteNth n l1) l2) :
-  { l3 & listIncl l1 l3 & listIncl l2 l3 } :=
-  pushoutListIncl (deleteNthIncl n l1) incl.
-
-Definition insertListIncl1 {A l1 l2} n a (incl : @listIncl1 A l1 l2) :
-  listIncl1 (insertNth a n l1) (insertNth a (applyListIncl1 incl n) l2).
-Proof.
-  revert n; induction incl; intros; [ | destruct n ].
-  - constructor.
-  - constructor; constructor; assumption.
-  - simpl. constructor. apply IHincl.
-Defined.
-
-Definition insertListIncl {A l1 l2} n a (incl : @listIncl A l1 l2) :
-  listIncl (insertNth a n l1) (insertNth a (applyListIncl incl n) l2).
-Proof.
-  revert n; induction incl; intros.
-  - constructor.
-  - apply stepListIncl; apply (insertListIncl1 n a incl).
-  - eapply compListIncl; [ apply IHincl1 | apply IHincl2 ].
-Defined.
-
-Definition insertListInclR {A} (a:A) n l : listIncl l (insertNth a n l).
-Proof.
-  apply stepListIncl; revert l; induction n; intro l;
-    [ | destruct l ]; constructor.
-  apply IHn.
-Defined.
-
-
 (** Event types **)
 
 (* An event type = a type of events plus their return types *)
-Polymorphic Record EvType@{u} : Type :=
-  { evTypeType :> Type@{u};
+Record EvType : Type :=
+  { evTypeType :> Type@{entree_u};
     evRetType : EncodingType evTypeType }.
 
-Global Instance EncodingType_EvType (ET:EvType) : EncodingType ET :=
-  evRetType ET.
+Global Instance EncodingType_EvType (E:EvType) : EncodingType E :=
+  evRetType E.
 
 (* The error event type *)
 Inductive ErrorE : Set :=
@@ -443,9 +58,15 @@ Global Instance EncodingType_ErrorE : EncodingType ErrorE := fun _ => Empty_set.
 
 (** Type Descriptions **)
 
-(* FIXME: if this approach works, we will want to make the kind and type
-descriptions extensible and/or instantiatable *)
+(* A type acts as a type description if it has a type of input and output types
+for functions *)
+Class IsTpDesc (Tp:Type@{entree_u}) : Type :=
+  { FunInput : Tp -> Type@{entree_u};
+    FunOutput : forall {T}, FunInput T -> Type@{entree_u};
+    dec_eq_Tp : forall (T U : Tp), {T=U} + {T<>U} }.
 
+
+(*
 (* Simple, non-dependent type descriptions *)
 Inductive SimpleDesc : Type@{entree_u} :=
 | SimpTp_Void : SimpleDesc
@@ -487,20 +108,15 @@ Proof.
   - destruct (IHT U) as [ e | neq ]; [ rewrite e; left; reflexivity | ].
     right; intro e; refine (neq _); inversion e; reflexivity.
 Admitted.
+*)
 
-(* Proof that a TpDesc is a monadic function type *)
-Fixpoint isFunTp (T:TpDesc) : Prop :=
-  match T with
-  | Tp_M _ => True
-  | Tp_Pi A B => forall a, isFunTp (B a)
-  | Tp_Arr A B => isFunTp B
-  | _ => False
-  end.
+Section FixTree.
 
+Context {Tp} `{IsTpDesc Tp} {E : EvType}.
 
 (* A "function index" is a monadic function referred to by index. It is
 essentially just a nat, but we make it a distinct type to make things clearer *)
-Inductive FunIx (T:TpDesc) : Type@{entree_u} :=
+Inductive FunIx (T:Tp) : Type@{entree_u} :=
 | MkFunIx (n:nat).
 
 Definition funIxIx {T} (f:FunIx T) : nat :=
@@ -508,6 +124,7 @@ Definition funIxIx {T} (f:FunIx T) : nat :=
   | MkFunIx _ n => n
   end.
 
+(*
 Fixpoint tpElem (T : TpDesc) : Type@{entree_u} :=
   match T with
   | Tp_M R => FunIx (Tp_M R)
@@ -537,17 +154,17 @@ Fixpoint FunOutputDesc T : FunInput T -> TpDesc :=
 
 Definition FunOutput T (args: FunInput T) : Type@{entree_u} :=
   tpElem (FunOutputDesc T args).
+*)
 
 
 (** Fun calls **)
 
-
 Inductive FunCall : Type@{entree_u} :=
-| MkFunCall T (f : FunIx T) (args : FunInput T).
+| MkFunCall (T:Tp) (f : FunIx T) (args : FunInput T).
 
 Definition FunCallRet (call: FunCall) :=
   match call with
-  | MkFunCall _ _ args => FunOutput _ args
+  | MkFunCall _ _ args => FunOutput args
   end.
 
 Global Instance EncodingType_FunCall : EncodingType FunCall := FunCallRet.
@@ -585,9 +202,6 @@ Definition unliftStackCallRet E stk U call :
 (**
  ** The definition of fixtrees
  **)
-Section fixtree.
-
-Context (E : EvType).
 
 (* The functor defining a single constructor of a fixtree *)
 Variant fixtreeF (F : Type@{entree_u} -> Type@{entree_u}) (R:Type@{entree_u}) : Type@{entree_u} :=
@@ -595,8 +209,8 @@ Variant fixtreeF (F : Type@{entree_u} -> Type@{entree_u}) (R:Type@{entree_u}) : 
   | Fx_TauF (t : F R)
   | Fx_VisF (e : E) (k : encodes e -> F R)
   | Fx_CallF (call : FunCall) (k : FunCallRet call -> F R)
-  | Fx_MkFunF (T : TpDesc)
-      (body : forall (args:FunInput T), F (FunOutput T args))
+  | Fx_MkFunF (T : Tp)
+      (body : forall (args:FunInput T), F (FunOutput args))
       (k : FunIx T -> F R)
 .
 
@@ -604,15 +218,13 @@ Variant fixtreeF (F : Type@{entree_u} -> Type@{entree_u}) (R:Type@{entree_u}) : 
 CoInductive fixtree R : Type@{entree_u} :=
   go { _fxobserve : fixtreeF fixtree R }.
 
-End fixtree.
-
 (* Implicit arguments and helpful notations for fixtrees *)
-Arguments Fx_RetF {_ _ _} _.
-Arguments Fx_TauF {_ _ _} _.
-Arguments Fx_VisF {_ _ _} _ _.
-Arguments Fx_CallF {_ _ _} _ _.
-Arguments Fx_MkFunF {_ _ _ _} _ _.
-Notation fixtree' E R := (fixtreeF E (fixtree E) R).
+Arguments Fx_RetF {_ _} _.
+Arguments Fx_TauF {_ _} _.
+Arguments Fx_VisF {_ _} _ _.
+Arguments Fx_CallF {_ _} _ _.
+Arguments Fx_MkFunF {_ _ _} _ _.
+Notation fixtree' R := (fixtreeF (fixtree) R).
 Notation Fx_Tau t := {| _fxobserve := Fx_TauF t |}.
 Notation Fx_Ret r := {| _fxobserve := Fx_RetF r |}.
 Notation Fx_Vis e k := {| _fxobserve := Fx_VisF e k |}.
@@ -620,20 +232,18 @@ Notation Fx_Call call k := {| _fxobserve := Fx_CallF call k |}.
 Notation Fx_MkFun body k := {| _fxobserve := Fx_MkFunF body k |}.
 
 (* "Observe" the top-most constructor of an fixtree by unwrapping it one step *)
-Definition fxobserve {E R} (t : fixtree E R) : fixtree' E R :=
-  _fxobserve _ _ t.
+Definition fxobserve {R} (t : fixtree R) : fixtree' R :=
+  _fxobserve _ t.
 
 
 (*** The basic operations on fixtrees ***)
 
-Module FixTree.
-
 (* This defines the bind operation by coinduction on the left-hand side of the
    bind; can also be seen as "substituting" an observed computation tree ot for
    the return value of a continuation k *)
-Definition subst' {E : EvType} {R S : Type@{entree_u}}
-           (k : R -> fixtree E S) : fixtree' E R -> fixtree E S  :=
-  cofix _subst (ot : fixtree' E R) :=
+Definition subst' {R S : Type@{entree_u}}
+           (k : R -> fixtree S) : fixtree' R -> fixtree S  :=
+  cofix _subst (ot : fixtree' R) :=
     match ot with
     | Fx_RetF r => k r
     | Fx_TauF t => Fx_Tau (_subst (fxobserve t))
@@ -643,18 +253,18 @@ Definition subst' {E : EvType} {R S : Type@{entree_u}}
     end.
 
 (* Wrap up subst' so it operates on an fixtree instead of an fixtree' *)
-Definition subst {E : EvType} {R S : Type@{entree_u}}
-           (k : R -> fixtree E S) : fixtree E R -> fixtree E S :=
+Definition subst {R S : Type@{entree_u}}
+           (k : R -> fixtree S) : fixtree R -> fixtree S :=
   fun t => subst' k (fxobserve t).
 
 (* Monadic bind for fixtrees is just subst *)
-Definition bind {E} {R S : Type@{entree_u}} 
-           (t : fixtree E R) (k : R -> fixtree E S) :=
+Definition bind {R S : Type@{entree_u}} 
+           (t : fixtree R) (k : R -> fixtree S) :=
   subst k t.
 
 (* Iterate a body on successive inputs of type I until it returns an R *)
-Definition iter {E} {I R : Type@{entree_u}}
-           (body : I -> fixtree E (I + R)) : I -> fixtree E R :=
+Definition iter {I R : Type@{entree_u}}
+           (body : I -> fixtree (I + R)) : I -> fixtree R :=
   cofix _iter i :=
     bind (body i) (fun ir => match ir with
                           | inl i' => Fx_Tau (_iter i')
@@ -662,52 +272,49 @@ Definition iter {E} {I R : Type@{entree_u}}
                           end).
 
 (* Map a pure function over the return value(s) of an entree *)
-Definition map {E} {R S} (f : R -> S) (t : fixtree E R) :=
+Definition map {R S} (f : R -> S) (t : fixtree R) :=
   bind t (fun r => Fx_Ret (f r)).
 
 (* Build a computation tree that performs a single event / effect in E *)
-Definition trigger {E:EvType} (e : E) : fixtree E (encodes e) :=
+Definition trigger (e : E) : fixtree (encodes e) :=
   Fx_Vis e (fun x => Fx_Ret x).
 
 (* The nonterminating computation that spins forever and never does anything *)
-CoFixpoint spin {E R} : fixtree E R := Fx_Tau spin.
+CoFixpoint spin {R} : fixtree R := Fx_Tau spin.
 
-End FixTree.
-
-CoFixpoint embedEntree' {E:EvType} {R} (ot: entree' E R) : fixtree E R :=
+CoFixpoint embedEntree' {R} (ot: entree' E R) : fixtree R :=
   match ot with
   | RetF r => Fx_Ret r
   | TauF t' => Fx_Tau (embedEntree' (observe t'))
   | VisF e k => Fx_Vis e (fun x => embedEntree' (observe (k x)))
   end.
 
-Definition embedEntree {E:EvType} {R} (t: entree E R) : fixtree E R :=
+Definition embedEntree {R} (t: entree E R) : fixtree R :=
   embedEntree' (observe t).
 
-Definition FxInterp E T :=
- forall (args:FunInput T), fixtree E (FunOutput T args).
+Definition FxInterp T := forall (args:FunInput T), fixtree (FunOutput args).
 
-Definition SomeFxInterp E := { T & FxInterp E T }.
+Definition SomeFxInterp := { T & FxInterp T }.
 
-Definition caseSomeFxInterp {E} T (d : SomeFxInterp E) : option (FxInterp E T) :=
-  match dec_eq_TpDesc (projT1 d) T with
-  | left e => Some (eq_rect (projT1 d) (FxInterp E) (projT2 d) T e)
+Definition caseSomeFxInterp T (d : SomeFxInterp) : option (FxInterp T) :=
+  match dec_eq_Tp (projT1 d) T with
+  | left e => Some (eq_rect (projT1 d) FxInterp (projT2 d) T e)
   | right _ => None
   end.
 
-Definition FxInterps E : Type@{entree_u} := list (SomeFxInterp E).
+Definition FxInterps : Type@{entree_u} := list SomeFxInterp.
 
-Definition nthSomeFxInterp {E} (defs : FxInterps E) n : option (SomeFxInterp E) :=
+Definition nthSomeFxInterp (defs : FxInterps) n : option SomeFxInterp :=
   nth_error defs n.
 
-Definition getFxInterp {E} (defs : FxInterps E) {T} (f : FunIx T) : option (FxInterp E T) :=
+Definition getFxInterp (defs : FxInterps) {T} (f : FunIx T) : option (FxInterp T) :=
   match nthSomeFxInterp defs (funIxIx f) with
   | Some d => caseSomeFxInterp T d
   | None => None
   end.
 
-Definition callFxInterp {E} (defs : FxInterps E) (call : FunCall)
-  : option (fixtree E (FunCallRet call)) :=
+Definition callFxInterp (defs : FxInterps) (call : FunCall)
+  : option (fixtree (FunCallRet call)) :=
   match call with
   | MkFunCall _ f args =>
       match getFxInterp defs f with
@@ -716,11 +323,11 @@ Definition callFxInterp {E} (defs : FxInterps E) (call : FunCall)
       end
   end.
 
-Definition consFxInterp {E} (defs : FxInterps E) {T} (d : FxInterp E T) : FxInterps E :=
-  app defs (existT (FxInterp E) T d :: nil).
+Definition consFxInterp (defs : FxInterps) {T} (d : FxInterp T) : FxInterps :=
+  app defs (existT FxInterp T d :: nil).
 
-CoFixpoint interp_fixtree' {E:EvType} {R} (err:entree E R) (defs : FxInterps E)
-  (ot : fixtree' E R) : entree E R :=
+CoFixpoint interp_fixtree' {R} (err:entree E R) (defs : FxInterps)
+  (ot : fixtree' R) : entree E R :=
   match ot with
   | Fx_RetF r => Ret r
   | Fx_TauF t => Tau (interp_fixtree' err defs (fxobserve t))
@@ -736,9 +343,25 @@ CoFixpoint interp_fixtree' {E:EvType} {R} (err:entree E R) (defs : FxInterps E)
              (fxobserve (k (MkFunIx _ (length defs)))))
   end.
 
-Definition interp_fixtree {E:EvType} {R}
-  (err:entree E R) (defs : FxInterps E) (t : fixtree E R) : entree E R :=
+Definition interp_fixtree {R} (err:entree E R) (defs : FxInterps) (t : fixtree R)
+  : entree E R :=
   interp_fixtree' err defs (fxobserve t).
+
+End FixTree.
+
+Arguments fixtree _ {_} _ _.
+Arguments fixtreeF _ {_} _ _.
+Arguments Fx_RetF {_ _ _ _ _} _.
+Arguments Fx_TauF {_ _ _ _ _} _.
+Arguments Fx_VisF {_ _ _ _ _} _ _.
+Arguments Fx_CallF {_ _ _ _ _} _ _.
+Arguments Fx_MkFunF {_ _ _ _ _ _} _ _.
+Notation fixtree' Tp E R := (fixtreeF Tp E (fixtree Tp E) R).
+Notation Fx_Tau t := {| _fxobserve := Fx_TauF t |}.
+Notation Fx_Ret r := {| _fxobserve := Fx_RetF r |}.
+Notation Fx_Vis e k := {| _fxobserve := Fx_VisF e k |}.
+Notation Fx_Call call k := {| _fxobserve := Fx_CallF call k |}.
+Notation Fx_MkFun body k := {| _fxobserve := Fx_MkFunF body k |}.
 
 
 (*** Notations for monadic computations ***)
@@ -760,10 +383,10 @@ End FixTreeNotations.
 
 (*** Instances to show that entrees form a monad ***)
 
-#[global] Instance Functor_fixtree {E} : Functor (fixtree E) :=
-  { fmap := @FixTree.map E }.
+#[global] Instance Functor_fixtree Tp `{IsTpDesc Tp} E : Functor (fixtree Tp E) :=
+  { fmap := @FixTree.map Tp _ E }.
 
-#[global] Instance Applicative_fixtree {E} : Applicative (fixtree E) :=
+#[global] Instance Applicative_fixtree Tp `{IsTpDesc Tp} E : Applicative (fixtree Tp E) :=
   {
     pure := fun _  x => Fx_Ret x;
     ap := fun _ _ f x =>
@@ -771,11 +394,11 @@ End FixTreeNotations.
 
   }.
 
-#[global] Instance Monad_fixtree {E} : Monad (fixtree E) :=
+#[global] Instance Monad_fixtree Tp `{IsTpDesc Tp} E : Monad (fixtree Tp E) :=
   {
     ret := fun _ x => Fx_Ret x;
-    bind := @FixTree.bind E;
+    bind := @FixTree.bind Tp _ E;
   }.
 
-#[global] Instance MonadIter_fixtree {E} : MonadIter (fixtree E) :=
+#[global] Instance MonadIter_fixtree Tp `{IsTpDesc Tp} E : MonadIter (fixtree Tp E) :=
   fun _ _ => FixTree.iter.
